some changes

examples/Example2_3.v
@@ -10,7 +10,7 @@ Require Import Morphisms.
 Local Open Scope string_scope.
 
 Definition M1 (p q: participant) (l: label): session :=
-  (p <-- ps_receive q [(l,isae(aevar "x"),ps_end)] | nilq) |||| (q <-- ps_send p l (isval (vint 42%Z)) ps_end | nilq).
+  (p <-- ps_receive q [(l,ps_end)] | nilq) |||| (q <-- ps_send p l (e_val (vint 42%Z)) ps_end | nilq).
 
 Definition M1' (p q: participant) (l: label): session :=
   (p <-- ps_end | nilq) |||| (q <-- ps_end | nilq).
@@ -20,14 +20,16 @@ Proof. intros.
        unfold beta_multistep, M1, M1'.
        setoid_rewrite scomm.
        apply multi_step with (y := 
-         ((q <-- ps_end | (conq nilq (mesq p l (vint 42) nilq))) ||||
-          (p <-- ps_receive q [(l, isae (aevar "x"), ps_end)] | nilq))).
-       apply r_send with (c := estate). simpl.
+         ((q <-- ps_end | (conq nilq (mesq p l (e_val (vint 42)) nilq))) ||||
+          (p <-- ps_receive q [(l,ps_end)] | nilq))).
+       apply r_send. simpl.
+       constructor.
+
        setoid_rewrite scomm.
        apply multi_step with (y := 
-         (((p <-- subst_expr (ps_receive q [(l, isae (aevar "x"), ps_end)]) l (isval (vint 42)) | nilq) |||| 
+         (((p <-- subst_expr_proc (ps_receive q [(l, ps_end)]) (e_val (vint 42)) l 0 0 | nilq) |||| 
           (q <-- ps_end | nilq)))).
-       specialize (r_rcv p q l ([(l, isae (aevar "x"), ps_end)])
+       specialize (r_rcv p q l ([(l, ps_end)])
                          (vint 42) (ps_end) nilq nilq
                          (p <-- ps_end | nilq)
        ); intro HR.
@@ -42,14 +44,14 @@ Qed.
 
 (* Example 2 in "A Very Gentle Introduction to Multiparty Session Types" *)
 Definition PAlice: process := 
-  ps_send "Bob" "l1" (isval (vint 50)) (ps_receive "Carol" [("l3",isae (aevar "x"),ps_end)]).
+  ps_send "Bob" "l1" (e_val (vnat 50)) (ps_receive "Carol" [("l3", ps_end)]).
 
 Definition PBob: process :=
-  ps_receive "Alice" [("l1",isae (aevar "x"),ps_send "Carol" "l2" (isval (vint 100)) ps_end); 
-                      ("l4",isae (aevar "x"),ps_send "Carol" "l2" (isval (vint 2))  ps_end)].
+  ps_receive "Alice" [("l1",ps_send "Carol" "l2" (e_val (vnat 100)) ps_end); 
+                      ("l4",ps_send "Carol" "l2" (e_val (vnat 2))  ps_end)].
 
 Definition PCarol: process :=
-  ps_receive "Bob" [("l2",isae (aevar "x"),ps_send "Alice" "l3" (isae (aesucc (aevar "x")))  ps_end)].
+  ps_receive "Bob" [("l2", ps_send "Alice" "l3" (e_succ (e_var 1))  ps_end)].
 
 Definition MS: session := ("Alice" <-- PAlice | nilq) |||| ("Bob" <-- PBob | nilq) |||| ("Carol" <-- PCarol | nilq).
 
@@ -59,10 +61,11 @@ Example redMS: beta_multistep MS MS'.
 Proof. intros.
        unfold beta_multistep, MS, MS', PAlice.
        apply multi_step with
-       (y := (("Alice" <-- (ps_receive "Carol" [("l3", isae (aevar "x"), ps_end)]) | conq nilq (mesq "Bob" "l1" (vint 50) nilq)) ||||
+       (y := (("Alice" <-- (ps_receive "Carol" [("l3", ps_end)]) | conq nilq (mesq "Bob" "l1" (e_val (vnat 50)) nilq)) ||||
              ("Bob" <-- PBob | nilq)) |||| ("Carol" <-- PCarol | nilq)).
        setoid_rewrite sassoc.
-       apply r_send with (c := estate). simpl.
+       apply r_send. simpl.
+       constructor.
 
        setoid_rewrite sassoc.
        setoid_rewrite scomm.
@@ -70,22 +73,23 @@ Proof. intros.
        setoid_rewrite <- sassoc.
 
        apply multi_step with
-       (y := ("Bob" <-- subst_expr (PBob) "l1" (isval (vint 50)) | nilq)
-              |||| ("Alice" <-- ps_receive "Carol" [("l3", isae (aevar "x"), ps_end)] | nilq)
+       (y := ("Bob" <-- subst_expr_proc (PBob) (e_val (vnat 50)) "l1"  0 0 | nilq)
+              |||| ("Alice" <-- ps_receive "Carol" [("l3", ps_end)] | nilq)
               |||| ("Carol" <-- PCarol | nilq)).
        apply r_rcv.
-       simpl. unfold exprR. 
+       simpl. 
        unfold PCarol.
 
        setoid_rewrite sassoc2.
        setoid_rewrite <- sassoc.
 
        apply multi_step with
-       (y := ((("Bob" <-- ps_end | conq nilq (mesq "Carol" "l2" (vint 100) nilq) )
-               |||| ("Carol" <-- ps_receive "Bob" [("l2", isae (aevar "x"), ps_send "Alice" "l3" (isae (aesucc (aevar "x"))) ps_end)] | nilq))
-               |||| ("Alice" <-- ps_receive "Carol" [("l3", isae (aevar "x"), ps_end)] | nilq))).
+       (y := ((("Bob" <-- ps_end | conq nilq (mesq "Carol" "l2" (e_val (vnat 100)) nilq) )
+               |||| ("Carol" <-- ps_receive "Bob" [("l2", ps_send "Alice" "l3" (e_succ (e_var 1)) ps_end)] | nilq))
+               |||| ("Alice" <-- ps_receive "Carol" [("l3", ps_end)] | nilq))).
        setoid_rewrite sassoc.
-       apply r_send with (c := estate). simpl.
+       apply r_send. simpl.
+       constructor.
 
        setoid_rewrite sassoc.
        setoid_rewrite scomm.
@@ -93,21 +97,22 @@ Proof. intros.
        setoid_rewrite <- sassoc.
 
        apply multi_step with
-       (y := ((("Carol" <-- subst_expr (ps_receive "Bob" [("l2", isae (aevar "x"), ps_send "Alice" "l3" (isae (aesucc (aevar "x")) ) ps_end)]) "l2" (isval (vint 100)) | nilq)
+       (y := ((("Carol" <-- subst_expr_proc (ps_receive "Bob" [("l2", ps_send "Alice" "l3" (e_succ (e_var 1)) ps_end)]) (e_val (vnat 100)) "l2" 0 0 | nilq)
                  |||| ("Bob" <-- ps_end | nilq))
-                 |||| ("Alice" <-- ps_receive "Carol" [("l3", isae (aevar "x"), ps_end)] | nilq))).
-       apply r_rcv. simpl. unfold exprR.
+                 |||| ("Alice" <-- ps_receive "Carol" [("l3", ps_end)] | nilq))).
+       apply r_rcv. simpl.
        simpl.
 
        setoid_rewrite sassoc2.
        setoid_rewrite <- sassoc.
 
        apply multi_step with
-       (y := ((("Carol" <-- ps_end | conq nilq (mesq "Alice" "l3" (eval estate (isae (aesucc (aeval 100)))) nilq) )
-               |||| ("Alice" <-- ps_receive "Carol" [("l3", isae (aevar "x"), ps_end)] | nilq))
+       (y := ((("Carol" <-- ps_end | conq nilq (mesq "Alice" "l3" (e_val (vnat 101)) nilq) )
+               |||| ("Alice" <-- ps_receive "Carol" [("l3", ps_end)] | nilq))
                |||| ("Bob" <-- ps_end | nilq))).
        setoid_rewrite sassoc.
-       apply r_send with (c := estate). simpl.
+       apply r_send. simpl.
+       specialize (ec_succ (e_val (vnat 100)) 100); intro He. apply He. constructor.
 
        setoid_rewrite sassoc.
        setoid_rewrite scomm.
@@ -115,14 +120,13 @@ Proof. intros.
        setoid_rewrite <- sassoc.
 
       apply multi_step with
-      (y := ((("Alice" <-- subst_expr (ps_receive "Carol" [("l3", isae (aevar "x"), ps_end)]) "l3" (isval (vint 101)) | nilq) 
+      (y := ((("Alice" <-- subst_expr_proc (ps_receive "Carol" [("l3", ps_end)]) (e_val (vnat 101)) "l3" 0 0 | nilq) 
              |||| ("Carol" <-- ps_end | nilq))
              |||| ("Bob" <-- ps_end | nilq))).
       apply r_rcv. simpl.
 
       apply multi_refl.
 Qed.
-
 
 
 
