processes/beta.v
@@ -1,3 +1,4 @@
+Require Import ST.processes.unscoped.
 Require Import ST.processes.axioms ST.processes.process.
 (* From mathcomp Require Import all_ssreflect seq. *)
 From Paco Require Import paco.
@@ -6,101 +7,73 @@ Local Open Scope string_scope.
 Import ListNotations.
 Require Import Setoid Morphisms.
 
-Definition veqb (v1 v2: value): bool :=
-  match (v1, v2) with
-    | (vint n1, vint n2  ) => Z.eqb n1 n2
-    | (vbool n1, vbool n2) => Bool.eqb n1 n2
-    | (vunit tt, vunit tt) => true
-    | _                    => false
-  end.
-
-Fixpoint aeeqb (e1 e2: aexpr): bool :=
-  match (e1, e2) with
-    | (aeval v1, aeval v2)   => Z.eqb v1 v2
-    | (aevar s1, aevar s2)   => eqb s1 s2
-    | (aesucc e1, aesucc e2) => aeeqb e1 e2
-    | (aeinv e1, aeinv e2)   => aeeqb e1 e2
-    | _                    => false
-  end.
-
-Fixpoint beeqb (e1 e2: bexpr): bool :=
-  match (e1, e2) with
-    | (beval v1, beval v2) => Bool.eqb v1 v2
-    | (bevar s1, bevar s2) => eqb s1 s2
-    | (beneg e1, beneg e2) => beeqb e1 e2
-    | _                    => false
-  end.
-
-Definition eeqb (e1 e2: expr): bool :=
-  match (e1, e2) with
-    | (isae v1, isae v2)   => aeeqb v1 v2
-    | (isbe v1, isbe v2)   => beeqb v1 v2
-    | (isgt v1, isgt v2)   => aeeqb v1 v2
-    | _                    => false
-  end.
-
-Definition total_map (A : Type) := string -> A.
-Definition state := total_map (Z*bool).
-Definition estate := fun (x: string) => (0%Z,false).
-
-Fixpoint aevaluate (m: state) (e: aexpr): Z :=
+Fixpoint incr_freeE (fv m : nat) (e : expr) :=
   match e with
-    | aeinv e1  => (aevaluate m e1) * (-1)
-    | aesucc e1 => (aevaluate m e1) + 1
-    | aevar x   => fst (m x) 
-    | aeval n   => n
+    | e_var n    => e_var (if Nat.leb fv n then (n + m) else n)
+    | e_val v    => e_val v 
+    | e_succ n   => e_succ (incr_freeE fv m n)
+    | e_neg n    => e_neg (incr_freeE fv m n)
+    | e_not n    => e_not (incr_freeE fv m n)
+    | e_gt u v   => e_gt (incr_freeE fv m u) (incr_freeE fv m v)
+    | e_plus u v => e_plus (incr_freeE fv m u) (incr_freeE fv m v) 
+    | e_det u v  => e_det (incr_freeE fv m u) (incr_freeE fv m v)
+  end. 
+
+Fixpoint subst_expr (n d : nat) (e : expr) (e1 : expr) : expr :=
+  match e1 with 
+    | e_var 0       => if Nat.eqb n 0 then (incr_freeE 0 d e) else e_var 0
+    | e_var (S m)   => if Nat.eqb (S m) n then (incr_freeE 0 d e) else 
+                       if Nat.ltb (S m) n then e_var (S m) else e_var m 
+    | e_succ e'     => e_succ (subst_expr n d e e')
+    | e_neg e'      => e_neg (subst_expr n d e e')
+    | e_not e'      => e_not (subst_expr n d e e')
+    | e_gt e' e''   => e_gt (subst_expr n d e e') (subst_expr n d e e'')
+    | e_plus e' e'' => e_plus (subst_expr n d e e') (subst_expr n d e e'')
+    | e_det e' e''  => e_det (subst_expr n d e e') (subst_expr n d e e'')
+    | _             => e1
   end.
 
-Definition negate(b: bool): bool :=
-  match b with
-    | true  => false
-    | false => true
+Fixpoint incr_free (fvP fvE m k : nat) (P : process) : process :=
+  match P with 
+    | ps_var n          => ps_var (if Nat.leb fvP n then (n + m) else n)
+    | ps_send p l e P'  => ps_send p l (incr_freeE fvE k e) (incr_free fvP fvE m k P')
+    | ps_receive p llp  => ps_receive p (List.map (
+                                                    fun u => match u with 
+                                                      | (l, p') => (l, (incr_free fvP (S fvE) m k p'))
+                                                    end) llp
+                                                  )
+    | ps_ite e P1 P2   => ps_ite (incr_freeE fvE k e) (incr_free fvP fvE m k P1) (incr_free fvP fvE m k P2)
+    | ps_mu P'         => ps_mu (incr_free (S fvP) fvE m k P')
+    | ps_inact         => ps_inact
   end.
 
-Fixpoint bevaluate (m: state) (e: bexpr): bool :=
-  match e with
-    | beneg e1  => negate (bevaluate m e1)
-    | bevar x   => snd (m x) 
-    | beval n   => n
+Fixpoint retProc (l: list(label*process)) (x: label): option process :=
+  match l with
+    | nil       => Datatypes.None
+    | (y,P)::ys => if eqb x y then Datatypes.Some P else retProc ys x
   end.
 
-Definition eval (m: state) (e: expr): value :=
-  match e with
-    | isae a  => vint (aevaluate m a)
-    | isbe b  => vbool (bevaluate m b)
-    | isgt e1 => vbool (Z.eqb (aevaluate m e1) 0)
-    | isval n => n 
+Fixpoint subst_expr_proc (p : process) (e : expr) (lb: label) (n d : nat) : process :=
+  match p with 
+    | ps_send pt l e' P => ps_send pt l (subst_expr n d e e') (subst_expr_proc P e lb n d)
+    | ps_ite e' P Q     => ps_ite (subst_expr n d e e') (subst_expr_proc P e lb n d) (subst_expr_proc Q e lb n d)
+    | ps_receive pt lst => (* ps_receive pt (map (fun x => match x with
+                                                          | (l, y) => if eqb l lb then (l, subst_expr_proc y e lb (S n) (S d)) else (l, y)
+                                                        end) lst) *)
+                           let fix next lst :=
+                           match lst with
+                             | nil         => p
+                             | (lbl,y)::xs => if eqb lbl lb then subst_expr_proc y e lb (S n) (S d) else next xs
+                           end
+                           in next lst
+    | ps_mu P           => ps_mu (subst_expr_proc P e lb n d)
+    | _ => p
   end.
 
-(*  Eval compute in
- eval (fun x => if eqb x "x" then (5%Z,false) else (0%Z,false)) (isae (aesucc (aesucc (aesucc (aevar "x"))))). *)
-
-Fixpoint aexprR (e: aexpr) (y: string) (e1: aexpr): aexpr :=
-  match e with
-    | aevar x   => if eqb x y then e1 else e
-    | aesucc e' => aesucc (aexprR e' y e1)
-    | aeinv e'  => aeinv (aexprR e' y e1)
-    | _         => e
-  end.
-
-Fixpoint bexprR (e: bexpr) (y: string) (e1: bexpr): bexpr :=
-  match e with
-    | bevar x   => if eqb x y then e1 else e
-    | beneg e'  => beneg (bexprR e' y e1)
-    | _        => e
-  end.
-
-Definition exprR (e: expr) (y: string) (e1: expr): expr :=
-  match (e,e1) with
-    | (isae a, isae a1)  => isae (aexprR a y a1)
-    | (isbe b, isbe b1)  => isbe (bexprR b y b1)
-    | (isgt a, isgt a1)  => isgt (aexprR a y a1)
-    | (isae a, isval (vint a1)) => isae (aexprR a y (aeval a1))
-    | (isbe a, isval (vbool a1)) => isbe (bexprR a y (beval a1))
-    | _                  => e
-  end.
-
-Fixpoint subst_expr (p: process) (l: label) (e: expr): process :=
+(* Compute (subst_expr_proc (ps_receive "Bob" (cons ("l2", 
+                          ps_send "Alice" "l3" (e_succ (e_var 1)) 
+                         (ps_send "Alice" "l4" (e_succ (e_var 1)) ps_end)) nil)) (e_val (vint 100)) "l2" 0 0). *)
+(* Fixpoint subst_expr (p: process) (l: label) (e: expr): process :=
   match p with
     | ps_receive s0 s1  => 
       let fix next lst :=
@@ -125,6 +98,7 @@ Fixpoint subst_expr (p: process) (l: label) (e: expr): process :=
      in next s1
     | _                                => p
   end.
+ *)
 
 Inductive qcong: relation mqueue :=
   | qcons : forall q1 q2 l1 l2 v1 v2 h1 h2, q1 <> q2 -> 
@@ -135,7 +109,7 @@ Inductive qcong: relation mqueue :=
   | qassoc: forall h1 h2 h3, qcong (conq h1 (conq h2 h3)) (conq (conq h1 h2) h3).
 
 Inductive pcong: relation process :=
-  | pmuUnf: forall p, pcong (ps_mu p) (unfold_muP p).
+  | pmuUnf: forall p, pcong (ps_mu p) (subst_process ((ps_mu p) .: ps_var) p).
 
 Inductive scong: relation session :=
   | sann   : forall p M, scong ((p <-- ps_end | nilq) |||| M) M
@@ -147,13 +121,21 @@ Inductive scong: relation session :=
                                    scong ((p <-- P | h1) |||| M) ((p <-- Q | h2) |||| M).
 
 Inductive beta: relation session :=
-  | r_send : forall p q l e P hp M c, beta ((p <-- (ps_send q l e P) | hp) |||| M) 
-                                           ((p <-- P | conq hp (mesq q l (eval c e) nilq)) |||| M)
-  | r_rcv   : forall p q l xs v Q hp hq M, beta ((p <-- ps_receive q xs | hp) |||| (q <-- Q | conq (mesq p l v nilq) hq) |||| M)
-                                                ((p <-- subst_expr (ps_receive q xs) l (isval v) | hp)  |||| (q <-- Q | hq) |||| M)
-  | r_cond_t: forall p e P Q h M c, eval c e = vbool true  -> beta ((p <-- ps_ite e P Q | h) |||| M) ((p <-- P | h) |||| M)
-  | r_cond_f: forall p e P Q h M c, eval c e = vbool false -> beta ((p <-- ps_ite e P Q | h) |||| M) ((p <-- Q | h) |||| M)
-  | r_struct: forall M1 M1' M2 M2', scong M1 M1' -> scong M2' M2 -> beta M1' M2' -> beta M1 M2.
+  | r_sendl  : forall p q l e P hp v, stepE e (e_val v) -> 
+                                      beta (p <-- (ps_send q l e P) | hp)
+                                           (p <-- P | conq hp (mesq q l (e_val v) nilq))
+  | r_rcvl   : forall p q l xs v Q hp hq, beta ((p <-- ps_receive q xs | hp) |||| (q <-- Q | conq (mesq p l (e_val v) nilq) hq))
+                                               ((p <-- subst_expr_proc (ps_receive q xs) (e_val v) l 0 0 | hp)  |||| (q <-- Q | hq))
+  | r_cond_tl: forall p e P Q h, stepE e (e_val (vbool true))  -> beta ((p <-- ps_ite e P Q | h)) ((p <-- P | h))
+  | r_cond_fl: forall p e P Q h, stepE e (e_val (vbool false)) -> beta ((p <-- ps_ite e P Q | h)) ((p <-- Q | h))
+  | r_send   : forall p q l e P hp M v, stepE e (e_val v) -> 
+                                        beta ((p <-- (ps_send q l e P) | hp) |||| M) 
+                                             ((p <-- P | conq hp (mesq q l (e_val v) nilq)) |||| M)
+  | r_rcv    : forall p q l xs v Q hp hq M, beta ((p <-- ps_receive q xs | hp) |||| (q <-- Q | conq (mesq p l (e_val v) nilq) hq) |||| M)
+                                                 ((p <-- subst_expr_proc (ps_receive q xs) (e_val v) l 0 0 | hp)  |||| (q <-- Q | hq) |||| M)
+  | r_cond_t : forall p e P Q h M, stepE e (e_val (vbool true))  -> beta ((p <-- ps_ite e P Q | h) |||| M) ((p <-- P | h) |||| M)
+  | r_cond_f : forall p e P Q h M, stepE e (e_val (vbool false)) -> beta ((p <-- ps_ite e P Q | h) |||| M) ((p <-- Q | h) |||| M)
+  | r_struct : forall M1 M1' M2 M2', scong M1 M1' -> scong M2' M2 -> beta M1' M2' -> beta M1 M2.
 
 Declare Instance Equivalence_beta : Equivalence beta.
 Declare Instance Equivalence_scong : Equivalence scong.
