types/typecheck.v
@@ -6,7 +6,7 @@ Require Import String List Datatypes ZArith.
 Local Open Scope string_scope.
 Import ListNotations.
 
-Inductive theta: Type :=
+(* Inductive theta: Type :=
   | tempt : theta
   | tconse: expr    -> local.sort -> theta -> theta
   | tconsp: process -> local      -> theta -> theta.
@@ -44,8 +44,9 @@ Definition is_ss (s1 s2: local.sort): bool :=
     | (sunit, sunit) => true
     | (snat, sint)   => true
     | _              => false
-  end.
+  end. *)
 
+(*
 Fixpoint tcAE (c: theta) (e: aexpr): option local.sort :=
   match e with
     | aeval n  => Some sint
@@ -71,7 +72,7 @@ Fixpoint tcBE (c: theta) (e: bexpr): option local.sort :=
                     | Some ss' => if sort_eqb ss' sbool then Some sbool else None 
                     | _        => None
                   end 
-  end.
+  end. *)
 
 (* Definition tcE (c: theta) (e: expr): option local.sort :=
   match e with
@@ -95,17 +96,123 @@ Definition stcE (c: theta) (e: expr) (S: local.sort): option local.sort :=
   end.
 *)
 
-Inductive tcE: theta -> expr -> local.sort -> Prop :=
+Definition ctxS := list (option local.sort).
+Definition ctxT := list (option local).
+
+Fixpoint SList {A} (lis : list A) : Prop := 
+  match lis with 
+    | x :: [] => True 
+    | _ :: xs                => SList xs
+    | []                     => False
+  end.
+
+Fixpoint extendLis {A} (n : nat) (ST : option A) : list (option A) :=
+  match n with 
+    | S m  => None :: extendLis m ST
+    | 0    => [ST]
+  end.
+
+Fixpoint onth {A : Type} (n : nat) (lis : list (option A)) : option A :=
+  match n with 
+    | S m => 
+      match lis with 
+        | x::xs => onth m xs
+        | []    => None 
+      end
+    | 0   =>
+      match lis with 
+        | x::xs => x 
+        | []    => None
+      end
+  end.
+
+Inductive typ_expr: ctxS -> expr -> local.sort -> Prop :=
+  | sc_var : forall c s t, onth s c = Some t -> typ_expr c (e_var s) t
+  | sc_vali: forall c i, typ_expr c (e_val (vint i)) sint
+  | sc_valn: forall c i, typ_expr c (e_val (vnat i)) snat
+  | sc_valb: forall c b, typ_expr c (e_val (vbool b)) sbool
+  | sc_succ: forall c e, typ_expr c e snat ->
+                         typ_expr c (e_succ e) snat
+  | sc_neg : forall c e, typ_expr c e sint ->
+                         typ_expr c (e_neg e) sint
+  | sc_sub : forall c e s s', typ_expr c e s ->
+                                 subsort s s' ->
+                                 typ_expr c e s'
+  | sc_not : forall c e, typ_expr c e sbool ->
+                         typ_expr c (e_not e) sbool
+  | sc_gt  : forall c e1 e2, typ_expr c e1 sint ->
+                             typ_expr c e2 sint ->
+                             typ_expr c (e_gt e1 e2) sbool
+  | sc_plus: forall c e1 e2, typ_expr c e1 sint ->
+                             typ_expr c e2 sint ->
+                             typ_expr c (e_plus e1 e2) sint
+  | sc_det  : forall c e1 e2 s, typ_expr c e1 s -> typ_expr c e2 s -> typ_expr c (e_det e1 e2) s.
+
+
+(* Inductive tcE: theta -> expr -> local.sort -> Prop :=
   | tce_iv1: forall c n, tcE c (isval (vint n)) sint
   | tce_iv2: forall c n, tcE c (isval (vbool n)) sbool
   | tce_iv3: forall c n, tcE c (isval (vunit n)) sunit
   | tce_iae: forall c a s, Some s = tcAE c a -> tcE c (isae a) sint
   | tce_ibe: forall c b s, Some s = tcBE c b -> tcE c (isbe b) sbool
   | tce_igt: forall c a s, Some s = tcAE c a -> tcE c (isgt a) sbool
-  | tce_iss: forall c e s' s, is_ss s s' = true -> tcE c e s' -> tcE c e s.
+  | tce_iss: forall c e s' s, is_ss s s' = true -> tcE c e s' -> tcE c e s. *)
 
 
-Fixpoint matchSel (l: label) (xs: list(label*local.sort*local)): option (local.sort*local) :=
+Inductive typ_proc: ctxS -> ctxT -> process -> local -> Prop :=
+  | tc_inact: forall cs ct,     typ_proc cs ct (ps_end) (lt_end)
+  | tc_var  : forall cs ct s t, nth s ct None = Some t -> (* wfC t -> *)
+                                typ_proc cs ct (ps_var s) t
+  | tc_mu   : forall cs ct p t,       typ_proc cs (Some t :: ct) p t ->
+                                      typ_proc cs ct (ps_mu p) t
+  | tc_ite  : forall cs ct e p1 p2 T, typ_expr cs e sbool ->
+                                      typ_proc cs ct p1 T ->
+                                      typ_proc cs ct p2 T ->
+                                      typ_proc cs ct (ps_ite e p1 p2) T
+  | tc_sst  : forall cs ct P T T' Tr Tr', typ_proc cs ct P T -> lt2stC T Tr -> lt2stC T' Tr' -> subtype3 Tr Tr'  -> typ_proc cs ct P T'
+  | tc_recv : forall cs ct p STT P,
+                     length P = length STT ->
+                     SList P ->
+                     Forall2 (fun u v => (exists l proc l' srt typ, u = (l, proc) /\ v = (l', srt, typ) /\ l = l' /\ typ_proc (Some srt :: cs) ct proc typ)) P STT ->
+                     typ_proc cs ct (ps_receive p P) (lt_receive p STT)
+  | tc_snd  : forall cs ct p l e P S T, typ_expr cs e S ->
+                                        typ_proc cs ct P T ->
+                                        typ_proc cs ct (ps_send p l e P) (lt_send p (cons (l, S, T) nil)).
+
+Lemma remark4_5: forall cs ct e, typ_expr cs e sbool ->
+                                 typ_proc cs ct (ps_ite e (ps_send "q" "l1" (e_val (vint 1%Z)) (ps_send "r" "l2" (e_val (vint 2)) ps_end)) 
+                                                          (ps_send "q" "l1" (e_val (vint 11)) (ps_send "r" "l2" (e_val (vint 22)) ps_end)))
+                                                (lt_send "q" [("l1",sint, lt_send "r" [("l2",sint,lt_end)])]).
+Proof. intros.
+       apply tc_ite.
+       - easy.
+       - specialize (tc_snd cs ct "q" "l1" (e_val (vint 1)) (ps_send "r" "l2" (e_val (vint 2)) ps_end) sint (lt_send "r" [("l2", sint, lt_end)])
+                    ); intro HS.
+         simpl in HS. apply HS; clear HS.
+         constructor.
+         specialize (tc_snd cs ct "r" "l2" (e_val (vint 2)) 
+                            (ps_end) sint
+                            (lt_end)
+                    ); intro HS.
+         simpl in HS. apply HS; clear HS.
+         constructor.
+         constructor.
+       - specialize (tc_snd cs ct "q" "l1" (e_val (vint 11)) 
+                            (ps_send "r" "l2" (e_val (vint 22)) ps_end) sint
+                            (lt_send "r" [("l2", sint, lt_end)])
+                    ); intro HS.
+         simpl in HS. apply HS; clear HS.
+         constructor.
+         specialize (tc_snd cs ct "r" "l2" (e_val (vint 22)) 
+                            (ps_end) sint
+                            (lt_end)
+                    ); intro HS.
+         simpl in HS. apply HS; clear HS.
+         constructor.
+         constructor.
+Qed.
+
+(* Fixpoint matchSel (l: label) (xs: list(label*local.sort*local)): option (local.sort*local) :=
   match xs with
     | nil           => None
     | (lbl,s,t)::ys => if eqb l lbl then Some(s,t) else matchSel l ys
@@ -124,9 +231,9 @@ Inductive tcP: theta -> process -> local -> Prop :=
                                     tcP c (ps_receive q (zip (zip L E) P)) (lt_receive q (zip (zip L S) T))
   | tc_condt: forall c e P Q T, tcE c e sbool -> tcP c P T -> tcP c Q T -> tcP c (ps_ite e P Q) T
   | tc_mu   : forall c P T, tcP (extendp c (ps_var 0) (lt_var 0)) P T -> tcP c (ps_mu P) (lt_mu T)
-  | tc_sst  : forall c P T T' Tr Tr', tcP c P T -> lt2stC T Tr -> lt2stC T' Tr' -> subtype3 Tr Tr'  -> tcP c P T'.
+  | tc_sst  : forall c P T T' Tr Tr', tcP c P T -> lt2stC T Tr -> lt2stC T' Tr' -> subtype3 Tr Tr'  -> tcP c P T'. *)
 
-Lemma remark4_5: forall c e, tcE c (isbe e) sbool ->
+(* Lemma remark4_5: forall c e, tcE c (isbe e) sbool ->
                              tcP c (ps_ite (isbe e) (ps_send "q" "l1" (isval (vint 1%Z)) (ps_send "r" "l2" (isval (vint 2)) ps_end)) 
                                                     (ps_send "q" "l1" (isval (vint 11)) (ps_send "r" "l2" (isval (vint 22)) ps_end)))
                                    (lt_send "q" [("l1",sint, lt_send "r" [("l2",sint,lt_end)])]).
@@ -168,7 +275,7 @@ Proof. intros.
          apply tce_iv1.
          apply tc_end.
 Qed.
-
+ *)
 
 
 
